base-thy/Data/Foldable.v
@@ -100,3 +100,55 @@ Proof.
   rewrite fold_left_app.
   auto.
 Qed.
+
+
+Lemma elem_nil : forall {A} `{Eq_ A}  (x:A),  
+  Foldable.elem x nil = false.
+Proof.
+  intros.
+  reflexivity.
+Qed.
+
+Lemma elem_cons : 
+  forall {A} `{Eq_ A} (v:A) (x:A) (l:list A),  
+    Foldable.elem v (x :: l) = (v == x) || Foldable.elem v l.
+Proof.
+  intros.
+  unfold Foldable.elem.
+  unfold Foldable.any.
+  unfold compose, SemigroupInternal.getAny, Foldable.foldMap.
+  unfold Foldable.Foldable__list,Foldable.foldMap__,
+  SemigroupInternal.Semigroup__Any,SemigroupInternal.Monoid__Any.
+  unfold Foldable.Foldable__list_foldMap. 
+  unfold Foldable.Foldable__list_foldr, mappend, mempty.
+  simpl.
+  f_equal.
+Qed.
+
+
+Lemma Foldable_any_app : forall {A} `{Eq_ A} (v:A) (l1 l2:list A),
+      Foldable.any (fun y : A => v == y) (l1 ++ l2) =
+      Foldable.any (fun y : A => v == y) l1
+      || Foldable.any (fun y : A => v == y) l2.
+Proof.
+  intros.
+  unfold Foldable.any.
+  unfold compose, Foldable.foldMap.
+  unfold Foldable.Foldable__list,Foldable.foldMap__,
+         Foldable.Foldable__list_foldMap,
+         Foldable.Foldable__list_foldr. 
+  simpl.
+  induction l1.
+  + simpl. auto.
+  + simpl.
+    rewrite <- orb_assoc.
+    f_equal.
+    unfold SemigroupInternal.getAny.
+    auto.
+Qed.
+
+Lemma Foldable_elem_app : forall {A}`{Eq_ A} (v:A) (l1 l2:list A),  
+    Foldable.elem v (l1 ++ l2) = Foldable.elem v l1 || Foldable.elem v l2.
+Proof.
+  intros. apply Foldable_any_app.
+Qed.
