base-thy/Data/Traversable.v
@@ -1,0 +1,75 @@
+Require Import GHC.Base.
+Require Import Data.Traversable.
+
+Require Import Proofs.GHC.Base.
+Require Import Proofs.GHC.List.
+
+From Coq Require Import ssreflect.
+Set Bullet Behavior "Strict Subproofs".
+
+
+
+(** [mapAccumL] instance for lists *)
+
+(*
+-- |The 'mapAccumL' function behaves like a combination of 'fmap'
+-- and 'foldl'; it applies a function to each element of a structure,
+-- passing an accumulating parameter from left to right, and returning
+-- a final value of this accumulator together with the new structure.
+mapAccumL :: Traversable t => (a -> b -> (a, c)) -> a -> t b -> (a, t c)
+mapAccumL f s t = runStateL (traverse (StateL . flip f) t) s *)
+
+(* 
+mapAccumL               :: (a -> b -> (a, c)) -> a -> [b] -> (a, [c])
+mapAccumL f s []        =  (s, [])
+mapAccumL f s (x:xs)    =  (s'',y:ys)
+                           where (s', y ) = f s x
+                                 (s'',ys) = mapAccumL f s' xs
+*)
+
+
+
+
+Lemma mapAccumL_nil : forall a b c  (f : a -> b -> (a * c)) (s : a), 
+   Traversable.mapAccumL f s nil = (s, nil).
+Proof.
+  intros a b c f s.
+  unfold Traversable.mapAccumL.
+  unfold Traversable.traverse,Traversable.Traversable__list, 
+         Traversable.traverse__ , 
+         Traversable.Traversable__list_traverse.
+  simpl.
+  auto.
+Qed.
+
+Lemma mapAccumL_cons : forall a b c x (xs : list b) (f : a -> b -> (a * c)) (s : a), 
+   Traversable.mapAccumL f s (cons x xs) = 
+   let '(s',y) := f s x in
+   let '(s'',ys) := Traversable.mapAccumL f s' xs in
+   (s'', cons y ys).
+Proof.
+  intros a b c x xs f s.
+  unfold Traversable.mapAccumL.
+  unfold Traversable.traverse,Traversable.Traversable__list, 
+         Traversable.traverse__ , 
+         Traversable.Traversable__list_traverse.
+  rewrite Base.hs_coq_foldr_base.
+  unfold op_z2218U__.
+  simpl.
+  unfold Utils.runStateL,liftA2, liftA2__, 
+  Utils.Applicative__StateL,Utils.Applicative__StateL_liftA2,
+  pure,pure__,Utils.Applicative__StateL_pure in *.
+  destruct (fold_right
+        (fun (x0 : b) (ys : Utils.StateL a (list c)) =>
+         match ys with
+         | Utils.Mk_StateL ky =>
+             Utils.Mk_StateL
+               (fun s0 : a =>
+                let
+                '(s', x1) := flip f x0 s0 in
+                 let '(s'', y) := ky s' in (s'', x1 :: y))
+         end) (Utils.Mk_StateL (fun s0 : a => (s0, nil))) xs) eqn:EQ.
+  unfold flip.
+  auto.
+Qed.
+
