examples/ghc/theories/VarEnv.v
@@ -1,0 +1,395 @@
+Require Import Coq.Lists.List.
+
+Require Import GHC.Base.
+Require Import Proofs.Data.Foldable.
+
+Require Import Id.
+Require Import Core.
+
+
+
+Require Import Proofs.Core.
+Require Import Proofs.Var.
+Require Import Proofs.Unique.
+Require Import Proofs.VarSet.
+
+Import GHC.Base.ManualNotations.
+
+Set Bullet Behavior "Strict Subproofs".
+
+
+(** ** [InScopeSet] *)
+
+Lemma getInScopeVars_extendInScopeSet:
+  forall iss v,
+  getInScopeVars (extendInScopeSet iss v) = extendVarSet (getInScopeVars iss) v.
+Proof.
+  intros.
+  unfold getInScopeVars.
+  unfold extendInScopeSet.
+  destruct iss.
+  reflexivity.
+Qed.
+
+Lemma getInScopeVars_extendInScopeSetList:
+  forall iss vs,
+  getInScopeVars (extendInScopeSetList iss vs) = extendVarSetList (getInScopeVars iss) vs.
+Proof.
+  intros.
+  unfold getInScopeVars.
+  unfold extendInScopeSetList.
+  set_b_iff.
+  destruct iss.
+  unfold_Foldable_foldl'.
+  unfold_Foldable_foldl.
+  f_equal.
+Qed.
+
+
+Lemma extendInScopeSetList_cons : forall v vs in_scope_set,
+           (extendInScopeSetList in_scope_set (v :: vs) = 
+            (extendInScopeSetList (extendInScopeSet in_scope_set v) vs)).
+Proof.
+  unfold extendInScopeSetList.
+  destruct in_scope_set.
+  unfold_Foldable_foldl.
+  simpl.
+  f_equal.
+  unfold Pos.to_nat.
+  unfold Pos.iter_op.
+  omega.
+Qed.
+
+Lemma extendInScopeSetList_nil : forall in_scope_set,
+           extendInScopeSetList in_scope_set nil = in_scope_set.
+Proof.
+  unfold extendInScopeSetList.
+  destruct in_scope_set.
+  unfold_Foldable_foldl.
+  simpl.
+  f_equal.
+  omega.
+Qed.
+
+Lemma lookupVarSet_extendVarSetList_l:
+  forall v vs1 vs2,
+  elemVarSet v (mkVarSet vs2) = false ->
+  lookupVarSet (extendVarSetList vs1 vs2) v = lookupVarSet vs1 v.
+Admitted.
+
+Lemma lookupVarSet_extendVarSetList_r_self:
+  forall v vs1 vs2,
+  List.In v vs2 ->
+  NoDup (map varUnique vs2) ->
+  lookupVarSet (extendVarSetList vs1 vs2) v = Some v.
+Admitted.
+
+
+(** ** [uniqAway] *)
+
+Axiom isJoinId_maybe_uniqAway:
+  forall s v, 
+  isJoinId_maybe (uniqAway s v) = isJoinId_maybe v.
+
+(* See discussion of [isLocalUnique] in [Proofs.Unique] *)
+Axiom isLocalUnique_uniqAway:
+  forall iss v,
+  isLocalUnique (varUnique (uniqAway iss v)) = true.
+
+Axiom isLocalId_uniqAway:
+  forall iss v,
+  isLocalId (uniqAway iss v) = isLocalId v.
+
+Axiom isLocalVar_uniqAway:
+  forall iss v,
+  isLocalVar (uniqAway iss v) = isLocalVar v.
+
+Lemma elemVarSet_uniqAway:
+  forall v iss vs,
+  subVarSet vs (getInScopeVars iss) = true ->
+  elemVarSet (uniqAway iss v) vs = false.
+Proof.
+  intros.
+  safe_unfold_VarSet.
+  destruct vs.
+  destruct iss.
+  destruct v0.
+  destruct u.
+  destruct u0.
+  simpl in *.
+  unfold uniqAway.
+  unfold elemInScopeSet.
+  unfold elemVarSet.
+  unfold uniqAway'.
+  unfold realUnique.
+Admitted.
+
+Axiom nameUnique_varName_uniqAway:
+  forall vss v,
+  Name.nameUnique (varName v) = varUnique v ->
+  Name.nameUnique (varName (uniqAway vss v)) = varUnique (uniqAway vss v).
+
+
+(** [uniqAway] axiomatization *)
+
+(* If uniqAway returns a variable with the same unique, 
+   it returns the same variable. *)      
+Axiom uniqAway_eq_same : forall v in_scope_set,
+    (uniqAway in_scope_set v == v) = true ->
+    (uniqAway in_scope_set v = v).
+
+(* The variable returned by uniqAway is fresh. *)
+Axiom uniqAway_lookupVarSet_fresh : forall v in_scope_set,
+    lookupVarSet (getInScopeVars in_scope_set) (uniqAway in_scope_set v) = None.
+
+
+
+
+
+(** [VarEnv] *)
+
+Axiom lookupVarEnv_elemVarEnv_true :
+  forall A v (vs : VarEnv A),
+   elemVarEnv v vs = true <-> (exists a, lookupVarEnv vs v = Some a).
+
+Axiom lookupVarEnv_elemVarEnv_false :
+  forall A v (vs : VarEnv A),
+   elemVarEnv v vs = false <-> (lookupVarEnv vs v = None).
+
+
+Axiom lookupVarEnv_eq :
+  forall A v1 v2 (vs : VarEnv A),
+    (v1 == v2) = true ->
+    lookupVarEnv vs v1 = lookupVarEnv vs v2.
+
+Axiom elemVarEnv_eq :
+  forall A v1 v2 (vs : VarEnv A),
+    (v1 == v2) = true ->
+    elemVarEnv v1 vs = elemVarEnv v2 vs.
+
+
+Axiom lookupVarEnv_extendVarEnv_eq :
+  forall A v1 v2 (vs : VarEnv A) val, 
+    v1 == v2 = true ->
+    lookupVarEnv (extendVarEnv vs v1 val) v2 = Some val.
+
+Axiom lookupVarEnv_extendVarEnv_neq :
+  forall A v1 v2 (vs : VarEnv A) val, 
+    v1 == v2 <> true ->
+    lookupVarEnv (extendVarEnv vs v1 val) v2 = lookupVarEnv vs v2.
+
+Axiom elemVarEnv_extendVarEnv_eq :
+  forall A v1 v2 (vs : VarEnv A) val, 
+    v1 == v2 = true ->
+    elemVarEnv v2 (extendVarEnv vs v1 val) = true.
+
+Axiom elemVarEnv_extendVarEnv_neq :
+  forall A v1 v2 (vs : VarEnv A) val, 
+    v1 == v2 <> true ->
+    elemVarEnv v2 (extendVarEnv vs v1 val) = elemVarEnv v2 vs.
+
+
+Axiom elemVarEnv_delVarEnv_eq :
+  forall A v1 v2 (vs : VarEnv A), 
+    v1 == v2 = true ->
+    elemVarEnv v2 (delVarEnv vs v1) = false.
+
+Axiom elemVarEnv_delVarEnv_neq :
+  forall A v1 v2 (env: VarEnv A), (v1 == v2) = false -> 
+               elemVarEnv v2 (delVarEnv env v1) = elemVarEnv v2 env.
+
+
+Axiom lookupVarEnv_delVarEnv_eq :
+  forall A v1 v2 (vs : VarEnv A), 
+    v1 == v2 = true ->
+    lookupVarEnv (delVarEnv vs v1) v2 = None.
+
+Axiom lookupVarEnv_delVarEnv_neq :
+  forall A v1 v2 (vs : VarEnv A), 
+    v1 == v2 <> true ->
+    lookupVarEnv (delVarEnv vs v1) v2 = lookupVarEnv vs v2.
+
+
+(** [minusDom] **)
+
+(* To be able to specify the property of a wellformed substitution, 
+   we need to define the operation of taking a variable set and 
+   removing all of the vars that are part of the domain of the 
+   substitution. *)
+
+
+Definition minusDom {a} (vs : VarSet) (e : VarEnv a) : VarSet :=
+  filterVarSet (fun v => negb (elemVarEnv v e)) vs.
+
+
+Ltac specialize_all var := 
+  repeat 
+    match goal with 
+    | [ H : forall var:Var, _ |- _ ] => specialize (H var)
+    end.
+
+(* After a case split on whether a var is present in a minusDom'ed env, 
+   rewrite a use of minusDom appropriately. *)
+Ltac rewrite_minusDom_true := 
+  match goal with 
+  | [ H : elemVarEnv ?var ?init_env = true |- 
+      context [ lookupVarSet 
+                  (minusDom ?s ?init_env) ?var ] ] =>  
+    unfold minusDom;
+    repeat rewrite lookupVarSet_filterVarSet_false with 
+        (f := (fun v0 : Var => negb (elemVarEnv v0 init_env ))); try rewrite H; auto 
+  | [ H : elemVarEnv ?var ?init_env = true, 
+          H2: context [ lookupVarSet 
+                          (minusDom ?s ?init_env) ?var ] |- _ ] =>  
+    unfold minusDom in H2;
+    rewrite lookupVarSet_filterVarSet_false with
+        (f := (fun v0 : Var => negb (elemVarEnv v0 init_env ))) in H2; 
+    try rewrite H; auto 
+                                                                    
+  end.
+
+Ltac rewrite_minusDom_false := 
+  match goal with 
+  | [ H : elemVarEnv ?var ?init_env  = false |- 
+      context [ lookupVarSet 
+                  (minusDom ?s ?init_env) ?var ] ] =>  
+    unfold minusDom;
+    repeat rewrite lookupVarSet_filterVarSet_true
+    with (f := (fun v0 : Var => negb (elemVarEnv v0 init_env ))); 
+    try rewrite H; auto 
+  | [ H : elemVarEnv ?var ?init_env = false, 
+          H2: context [ lookupVarSet 
+                          (minusDom ?s ?init_env) ?var ] |- _ ] =>  
+    unfold minusDom in H2;
+    rewrite lookupVarSet_filterVarSet_true with 
+        (f := (fun v0 : Var => negb (elemVarEnv v0 init_env ))) in H2 ; 
+    try rewrite H; auto  
+  end.
+
+
+Lemma StrongSubset_minusDom {a} : forall vs1 vs2 (e: VarEnv a), 
+    vs1 {<=} vs2 ->
+    minusDom vs1 e {<=} minusDom vs2 e.
+Proof.
+  intros. 
+  unfold StrongSubset in *.
+  intros var.
+  destruct (elemVarEnv var e) eqn:IN_ENV.
+  + rewrite_minusDom_true. 
+  + rewrite_minusDom_false.
+    eapply H.
+Qed.
+
+
+Lemma lookupVarSet_minusDom_1 :
+  forall a (env : VarEnv a) vs v,
+    lookupVarEnv env v = None -> 
+    lookupVarSet (minusDom vs env) v = lookupVarSet vs v.
+Proof.
+  intros.
+  rewrite <- lookupVarEnv_elemVarEnv_false in H.
+  unfold minusDom.
+  rewrite lookupVarSet_filterVarSet_true
+    with (f := (fun v0 : Var => negb (elemVarEnv v0 env))).
+  auto.
+  rewrite H. simpl. auto.
+Qed.
+
+
+
+Lemma lookup_minusDom_inDom : forall a vs (env:VarEnv a) v',
+    elemVarEnv v' env = true ->
+    lookupVarSet (minusDom vs env) v' = None.
+Proof.
+  intros.
+  rewrite_minusDom_true.
+Qed. 
+
+
+Lemma minusDom_extend : 
+  forall a vs (env : VarEnv a) v,
+    minusDom (extendVarSet vs v) (delVarEnv env v) {<=} 
+    extendVarSet (minusDom vs env) v.
+Proof.
+  intros.
+  unfold StrongSubset.
+  intros var.
+  destruct (elemVarEnv var (delVarEnv env v)) eqn:IN.
+  rewrite_minusDom_true.
+  rewrite_minusDom_false.
+  destruct (v == var) eqn:EQ.
+  rewrite lookupVarSet_extendVarSet_eq;auto.
+  rewrite lookupVarSet_extendVarSet_eq; auto.
+  eapply almostEqual_refl; auto.
+  rewrite lookupVarSet_extendVarSet_neq; auto.
+  destruct (lookupVarSet vs var) eqn:IN2; auto.
+  rewrite lookupVarSet_extendVarSet_neq; auto.
+  rewrite lookupVarSet_filterVarSet_true; try rewrite IN; auto.
+  rewrite IN2.
+  apply almostEqual_refl; auto.
+  rewrite elemVarEnv_delVarEnv_neq in IN; auto.
+  rewrite IN. auto.
+  intro h. rewrite h in EQ. discriminate.
+  intro h. rewrite h in EQ. discriminate.
+Qed.
+
+
+Lemma lookup_minusDom_extend : forall a vs (env:VarEnv a) v v' e,
+    v ==  v' <> true ->
+    lookupVarSet (minusDom (extendVarSet vs v) (extendVarEnv env v e)) v' =
+    lookupVarSet (minusDom vs env) v'.
+Proof.
+  intros.
+  destruct (elemVarEnv v' env) eqn:Eenv; auto.
+  + (* v' is in dom of env. so cannot be looked up. *)
+    unfold minusDom.
+    rewrite 2 lookupVarSet_filterVarSet_false; auto.  
+    rewrite Eenv. simpl. auto.
+    rewrite elemVarEnv_extendVarEnv_neq.
+    rewrite Eenv. simpl. auto.
+    auto.
+  + unfold minusDom.
+    rewrite 2 lookupVarSet_filterVarSet_true; auto.  
+    rewrite lookupVarSet_extendVarSet_neq; auto.
+    auto.
+    rewrite Eenv. simpl. auto.
+    rewrite elemVarEnv_extendVarEnv_neq.
+    rewrite Eenv. simpl. auto.
+    auto.
+Qed.
+
+Lemma StrongSubset_minusDom_left {a} : forall vs (e: VarEnv a), 
+    minusDom vs e {<=} vs.
+Proof.
+  intros.
+  unfold StrongSubset. intro var.
+  destruct (elemVarEnv var e) eqn:EL.
+  rewrite_minusDom_true.
+  rewrite_minusDom_false.
+  destruct lookupVarSet.
+  eapply almostEqual_refl.
+  auto.
+Qed.
+
+
+Lemma StrongSubset_minusDom_extend_extend : forall vs v e (env: IdEnv CoreExpr),
+           minusDom (extendVarSet vs v) (extendVarEnv env v e) {<=} minusDom vs env.
+Proof.
+  intros.
+  intro var.
+  destruct (var == v) eqn:EQ.
+  rewrite lookupVarSet_eq with (v2 := v); auto.
+  unfold minusDom.
+  rewrite lookupVarSet_filterVarSet_false. 
+  auto.
+  rewrite elemVarEnv_extendVarEnv_eq.
+  simpl. auto.
+  rewrite Base.Eq_refl. auto.
+  rewrite lookup_minusDom_extend.
+  destruct (lookupVarSet (minusDom vs env) var).
+  eapply almostEqual_refl. auto.
+  intro h.
+  rewrite Base.Eq_sym in h.
+  rewrite h in EQ.
+  discriminate.
+Qed.
